Better names for basic examples.

theories/examples/basics.v
@@ -5,17 +5,17 @@ From iris.heap_lang Require Import proofmode notation lib.spin_lock.
 From actris.utils Require Import contribution.
 
 (** Basic *)
-Definition prog1 : val := λ: <>,
+Definition prog : val := λ: <>,
   let: "c" := start_chan (λ: "c'", send "c'" #42) in
   recv "c".
 
 (** Tranfering References *)
-Definition prog1_ref : val := λ: <>,
+Definition prog_ref : val := λ: <>,
   let: "c" := start_chan (λ: "c'", send "c'" (ref #42)) in
   ! (recv "c").
 
 (** Delegation, i.e. transfering channels *)
-Definition prog1_del : val := λ: <>,
+Definition prog_del : val := λ: <>,
   let: "c1" := start_chan (λ: "c1'",
     let: "cc2" := new_chan #() in
     send "c1'" (Fst "cc2");;
@@ -23,18 +23,18 @@ Definition prog1_del : val := λ: <>,
   recv (recv "c1").
 
 (** Dependent protocols *)
-Definition prog2 : val := λ: <>,
+Definition prog_dep : val := λ: <>,
   let: "c" := start_chan (λ: "c'",
     let: "x" := recv "c'" in send "c'" ("x" + #2)) in
   send "c" #40;;
   recv "c".
 
-Definition prog2_ref : val := λ: <>,
+Definition prog_dep_ref : val := λ: <>,
   let: "c" := start_chan (λ: "c'",
     let: "l" := recv "c'" in "l" <- !"l" + #2;; send "c'" #()) in
   let: "l" := ref #40 in send "c" "l";; recv "c";; !"l".
 
-Definition prog2_del : val := λ: <>,
+Definition prog_dep_del : val := λ: <>,
   let: "c1" := start_chan (λ: "c1'",
     let: "cc2" := new_chan #() in
     send "c1'" (Fst "cc2");;
@@ -42,7 +42,7 @@ Definition prog2_del : val := λ: <>,
   let: "c2'" := recv "c1" in send "c2'" #40;; recv "c2'".
 
 (** Transfering higher-order functions *)
-Definition prog3 : val := λ: <>,
+Definition prog_fun : val := λ: <>,
   let: "c" := start_chan (λ: "c'",
     let: "f" := recv "c'" in send "c'" (λ: <>, "f" #() + #2)) in
   let: "r" := ref #40 in
@@ -61,27 +61,27 @@ Section proofs.
 Context `{heapG Σ, proto_chanG Σ}.
 
 (** Protocols for the respective programs *)
-Definition prot1 : iProto Σ :=
+Definition prot : iProto Σ :=
   (<?> MSG #42; END)%proto.
 
-Definition prot1_ref : iProto Σ :=
+Definition prot_ref : iProto Σ :=
   (<?> l : loc, MSG #l {{ l ↦ #42 }}; END)%proto.
 
-Definition prot1_del : iProto Σ :=
-  (<?> c : val, MSG c {{ c ↣ prot1 }}; END)%proto.
+Definition prot_del : iProto Σ :=
+  (<?> c : val, MSG c {{ c ↣ prot }}; END)%proto.
 
-Definition prot2 : iProto Σ :=
+Definition prot_dep : iProto Σ :=
   (<!> x : Z, MSG #x; <?> MSG #(x + 2); END)%proto.
 
-Definition prot2_ref : iProto Σ :=
+Definition prot_dep_ref : iProto Σ :=
   (<!> (l : loc) (x : Z), MSG #l {{ l ↦ #x }};
    <?> MSG #() {{ l ↦ #(x + 2) }};
    END)%proto.
 
-Definition prot2_del : iProto Σ :=
-  (<?> c : val, MSG c {{ c ↣ prot2 }}; END)%proto.
+Definition prot_dep_del : iProto Σ :=
+  (<?> c : val, MSG c {{ c ↣ prot_dep }}; END)%proto.
 
-Definition prot3 : iProto Σ :=
+Definition prot_fun : iProto Σ :=
   (<!> (P : iProp Σ) (Φ : Z → iProp Σ) (vf : val),
      MSG vf {{ {{{ P }}} vf #() {{{ x, RET #x; Φ x }}} }};
    <?> (vg : val),
@@ -95,64 +95,64 @@ Fixpoint prot_lock (n : nat) : iProto Σ :=
   end%proto.
 
 (** Specs and proofs of the respective programs *)
-Lemma prog1_spec : {{{ True }}} prog1 #() {{{ RET #42; True }}}.
+Lemma prog_spec : {{{ True }}} prog #() {{{ RET #42; True }}}.
 Proof.
   iIntros (Φ) "_ HΦ". wp_lam.
-  wp_apply (start_chan_proto_spec prot1); iIntros (c) "Hc".
+  wp_apply (start_chan_proto_spec prot); iIntros (c) "Hc".
   - by wp_send with "[]".
   - wp_recv as "_". by iApply "HΦ".
 Qed.
 
-Lemma prog1_ref_spec : {{{ True }}} prog1_ref #() {{{ RET #42; True }}}.
+Lemma prog_ref_spec : {{{ True }}} prog_ref #() {{{ RET #42; True }}}.
 Proof.
   iIntros (Φ) "_ HΦ". wp_lam.
-  wp_apply (start_chan_proto_spec prot1_ref); iIntros (c) "Hc".
+  wp_apply (start_chan_proto_spec prot_ref); iIntros (c) "Hc".
   - wp_alloc l as "Hl". by wp_send with "[$Hl]".
   - wp_recv (l) as "Hl". wp_load. by iApply "HΦ".
 Qed.
 
-Lemma prog1_del_spec : {{{ True }}} prog1_del #() {{{ RET #42; True }}}.
+Lemma prog_del_spec : {{{ True }}} prog_del #() {{{ RET #42; True }}}.
 Proof.
   iIntros (Φ) "_ HΦ". wp_lam.
-  wp_apply (start_chan_proto_spec prot1_del); iIntros (c) "Hc".
+  wp_apply (start_chan_proto_spec prot_del); iIntros (c) "Hc".
   - wp_apply (new_chan_proto_spec with "[//]").
-    iIntros (c2 c2') "Hcc2". iMod ("Hcc2" $! prot1) as "[Hc2 Hc2']".
+    iIntros (c2 c2') "Hcc2". iMod ("Hcc2" $! prot) as "[Hc2 Hc2']".
     wp_send with "[$Hc2]". by wp_send with "[]".
   - wp_recv (c2) as "Hc2". wp_recv as "_". by iApply "HΦ".
 Qed.
 
-Lemma prog2_spec : {{{ True }}} prog2 #() {{{ RET #42; True }}}.
+Lemma prog_dep_spec : {{{ True }}} prog_dep #() {{{ RET #42; True }}}.
 Proof.
   iIntros (Φ) "_ HΦ". wp_lam.
-  wp_apply (start_chan_proto_spec prot2); iIntros (c) "Hc".
+  wp_apply (start_chan_proto_spec prot_dep); iIntros (c) "Hc".
   - wp_recv (x) as "_". by wp_send with "[]".
   - wp_send with "[//]". wp_recv as "_". by iApply "HΦ".
 Qed.
 
-Lemma prog2_ref_spec : {{{ True }}} prog2_ref #() {{{ RET #42; True }}}.
+Lemma prog2_ref_spec : {{{ True }}} prog_dep_ref #() {{{ RET #42; True }}}.
 Proof.
   iIntros (Φ) "_ HΦ". wp_lam.
-  wp_apply (start_chan_proto_spec prot2_ref); iIntros (c) "Hc".
+  wp_apply (start_chan_proto_spec prot_dep_ref); iIntros (c) "Hc".
   - wp_recv (l x) as "Hl". wp_load. wp_store. by wp_send with "[Hl]".
   - wp_alloc l as "Hl". wp_send with "[$Hl]". wp_recv as "Hl". wp_load.
     by iApply "HΦ".
 Qed.
 
-Lemma prog2_del_spec : {{{ True }}} prog2_del #() {{{ RET #42; True }}}.
+Lemma prog_dep_del_spec : {{{ True }}} prog_dep_del #() {{{ RET #42; True }}}.
 Proof.
   iIntros (Φ) "_ HΦ". wp_lam.
-  wp_apply (start_chan_proto_spec prot2_del); iIntros (c) "Hc".
+  wp_apply (start_chan_proto_spec prot_dep_del); iIntros (c) "Hc".
   - wp_apply (new_chan_proto_spec with "[//]").
-    iIntros (c2 c2') "Hcc2". iMod ("Hcc2" $! prot2) as "[Hc2 Hc2']".
+    iIntros (c2 c2') "Hcc2". iMod ("Hcc2" $! prot_dep) as "[Hc2 Hc2']".
     wp_send with "[$Hc2]". wp_recv (x) as "_". by wp_send with "[]".
   - wp_recv (c2) as "Hc2". wp_send with "[//]". wp_recv as "_".
     by iApply "HΦ".
 Qed.
 
-Lemma prog3_spec : {{{ True }}} prog3 #() {{{ RET #42; True }}}.
+Lemma prog_fun_spec : {{{ True }}} prog_fun #() {{{ RET #42; True }}}.
 Proof.
   iIntros (Φ) "_ HΦ". wp_lam.
-  wp_apply (start_chan_proto_spec prot3); iIntros (c) "Hc".
+  wp_apply (start_chan_proto_spec prot_fun); iIntros (c) "Hc".
   - wp_recv (P Ψ vf) as "#Hf". wp_send with "[]"; last done.
     iIntros "!>" (Ψ') "HP HΨ'". wp_apply ("Hf" with "HP"); iIntros (x) "HΨ".
     wp_pures. by iApply "HΨ'".
